compilationhelper.dfy
@@ -1,0 +1,820 @@
+include "lemmas.dfy"
+include "common.dfy"
+include "steps.dfy"
+include "equivalence.dfy"
+include "triviallemmas.dfy"
+include "loops.dfy"
+
+
+module CompilationHelper{
+    import opened Lemmas
+    import opened Common
+    import opened Steps
+    import opened Equivalence
+    import opened Trivial
+    import opened Loops
+
+    method AddElementToStack(loop: seq<int>, commands: seq<Instr>) returns (result: seq<int>)
+    requires loop_less_than_commands(loop, commands)
+    requires |commands| > 0
+    requires commands[|commands|-1] == Jump(0, true)
+    ensures loop_less_than_commands(result, commands)
+
+    {
+    result := loop;
+    assert loop_less_than_commands(result, commands);
+    result := result + [|commands|-1];
+    assert loop_less_than_commands(result, commands);
+    }
+
+    method CompilePlus(p: Program, commands: seq<Instr>, i: int, next_command_indices: seq<int>, j: int, old_i: int, loop_start_stack: seq<int>) 
+    returns (result: seq<Instr>, new_index: int)
+    requires i >= 0
+    requires valid_program(p)
+    requires next_command_indices == Changes(p)
+    requires |p.commands| > 0
+    requires |p.input| == |p.commands|
+    requires p.pointer == 0
+    requires valid_input(p.input)
+    requires |commands|>=0
+    requires changes_correct(p, next_command_indices)
+    requires sub_changes_inclusion_1_step(p, next_command_indices)
+    requires inside_the_indices(p, next_command_indices, i) //i is either greater than |p.commands| or i is in the indices
+    requires 0<=j < |next_command_indices|
+    requires j < |next_command_indices| ==> next_command_indices[j]==i
+    requires i >= |p.commands| ==> !(i in next_command_indices)
+    requires i >= |p.commands| ==> j >= |next_command_indices|
+    requires j == |commands|
+    requires old_i == i
+    requires p.commands[next_command_indices[j]] == '+'
+    requires matched_forall_loop(p, commands, next_command_indices, j)
+    requires in_bounds_commands(p, next_command_indices)
+    requires loop_less_than_commands(loop_start_stack, commands)
+    requires valid_ir_commands(commands)
+    ensures |result| == |commands|+1
+    ensures j < |result| && j < |next_command_indices|
+    ensures matched_command_with_ir(p, result, j, next_command_indices)
+    ensures matched_forall_loop(p, result, next_command_indices, j+1)
+    ensures in_bounds_commands(p, next_command_indices)
+    ensures loop_less_than_commands(loop_start_stack, result)
+    ensures valid_ir_commands(result)
+    ensures loop_less_than_commands(loop_start_stack, result)
+    ensures j== |result|-1
+    ensures matched_forall_loop(p, result, next_command_indices, j+1)
+    ensures in_bounds_commands(p, next_command_indices)
+    ensures old_i in next_command_indices ==> inside_the_indices(p, next_command_indices, new_index)
+    ensures inside_the_indices(p, next_command_indices, new_index)
+    ensures j+1 <= |next_command_indices| ==> j < |next_command_indices|
+    ensures matched_forall_loop(p, result, next_command_indices, j)
+    ensures |result| >0
+    ensures relation_between_old_new(p, old_i, new_index, next_command_indices)
+    ensures new_index >= 0
+    ensures inside_the_indices(p, next_command_indices, new_index) //new_index is either greater than |p.commands| or new_index is in the indices
+    ensures new_index >= |p.commands| ==> !(new_index in next_command_indices)
+    ensures j+1 <= |next_command_indices|
+    ensures j+1 == |result|
+    ensures j+1 < |next_command_indices| ==> next_command_indices[j+1]==new_index
+    ensures matched_forall_loop(p, result, next_command_indices, j)
+    ensures in_bounds_commands(p, next_command_indices)
+    ensures loop_less_than_commands(loop_start_stack, result)
+    ensures valid_ir_commands(result)
+    ensures new_index >= 0
+    ensures |commands| >=0
+    ensures sub_changes_inclusion_1_step(p, next_command_indices)
+    ensures inside_the_indices(p, next_command_indices, new_index)
+    ensures new_index > i
+
+
+    {
+        assert matched_forall_loop(p, commands, next_command_indices, j);
+        var k:= count_consecutive_symbols(p, i);
+        implication_with_and(p, i, k, next_command_indices); 
+        assert (i in next_command_indices && next_step(p, i, k, next_command_indices)) ==> inside_the_indices(p, next_command_indices, i+k);
+        assert i in next_command_indices ==> next_step(p, i, k, next_command_indices);
+        step_is_indices(p, i, k, next_command_indices);
+        assert (i in next_command_indices) ==> inside_the_indices(p, next_command_indices, i+k);
+        assert matched_forall_loop(p, commands, next_command_indices, j);
+        
+        assert valid_ir_commands(commands);
+        result := commands+ [Inc(k)]; 
+
+        assert valid_ir_commands(result[..|result|-1]);
+        IncreasingArrayKeepsValid(result);
+        assert valid_ir_commands(result);
+
+        assert matched_forall_loop(p, result[..j], next_command_indices, j);
+        IncreasingArrayDoesntAffectMatching(p, result, j, next_command_indices);
+        assert matched_forall_loop(p, result, next_command_indices, j);
+        // assume false;
+
+        assert |result| >0;
+        assert (old_i in next_command_indices) ==> inside_the_indices(p, next_command_indices, i+k);
+        assert relation_between_old_new(p, old_i, i+k, next_command_indices);
+        var temp := i+k;      
+        addition_is_preserving(p, old_i, i, k, temp, next_command_indices);
+        assert relation_between_old_new(p, old_i, temp, next_command_indices);
+
+        // i := temp;
+        assert temp-old_i == k;
+        assert (old_i in next_command_indices) ==> inside_the_indices(p, next_command_indices, temp);
+        assert p.commands[next_command_indices[j]] == '+';
+        assert k == count_consecutive_symbols(p, next_command_indices[j]);
+        assert k >= 0;
+        assert result[j] == Inc(k);
+        AndIsImplicationPlus(p, result, j, next_command_indices, k);
+        assert matched_command_with_ir(p, result, j, next_command_indices);
+        assert matched_forall_loop(p, result, next_command_indices, j+1);
+        assert in_bounds_commands(p, next_command_indices);
+        assert loop_less_than_commands(loop_start_stack, result);
+        new_index := temp;
+        assert just_short_length(j, next_command_indices) ==> next_command_indices[j+1] == next_command_indices[j] + count_consecutive_symbols(p, next_command_indices[j]);
+        assert j+1 < |next_command_indices| ==> next_command_indices[j+1] == i + k;
+        assert j +1 < |next_command_indices| ==> next_command_indices[j+1] == new_index;
+
+    }
+
+
+    method CompileMinus(p: Program, commands: seq<Instr>, i: int, next_command_indices: seq<int>, j: int, old_i: int, loop_start_stack: seq<int>) 
+    returns (result: seq<Instr>, new_index: int)
+    requires i >= 0
+    requires valid_program(p)
+    requires next_command_indices == Changes(p)
+    requires |p.commands| > 0
+    requires |p.input| == |p.commands|
+    requires p.pointer == 0
+    requires valid_input(p.input)
+    requires |commands|>=0
+    requires changes_correct(p, next_command_indices)
+    requires sub_changes_inclusion_1_step(p, next_command_indices)
+    requires inside_the_indices(p, next_command_indices, i) //i is either greater than |p.commands| or i is in the indices
+    requires 0<=j < |next_command_indices|
+    requires j < |next_command_indices| ==> next_command_indices[j]==i
+    requires i >= |p.commands| ==> !(i in next_command_indices)
+    requires i >= |p.commands| ==> j >= |next_command_indices|
+    requires j == |commands|
+    requires old_i == i
+    requires p.commands[next_command_indices[j]] == '-'
+    requires matched_forall_loop(p, commands, next_command_indices, j)
+    requires in_bounds_commands(p, next_command_indices)
+    requires loop_less_than_commands(loop_start_stack, commands)
+    requires valid_ir_commands(commands)
+    ensures |result| == |commands|+1
+    ensures j < |result| && j < |next_command_indices|
+    ensures matched_command_with_ir(p, result, j, next_command_indices)
+    ensures matched_forall_loop(p, result, next_command_indices, j+1)
+    ensures in_bounds_commands(p, next_command_indices)
+    ensures loop_less_than_commands(loop_start_stack, result)
+    ensures valid_ir_commands(result)
+    ensures loop_less_than_commands(loop_start_stack, result)
+    ensures j== |result|-1
+    ensures matched_forall_loop(p, result, next_command_indices, j+1)
+    ensures in_bounds_commands(p, next_command_indices)
+    ensures old_i in next_command_indices ==> inside_the_indices(p, next_command_indices, new_index)
+    ensures inside_the_indices(p, next_command_indices, new_index)
+    ensures j+1 <= |next_command_indices| ==> j < |next_command_indices|
+    ensures matched_forall_loop(p, result, next_command_indices, j)
+    ensures |result| >0
+    ensures relation_between_old_new(p, old_i, new_index, next_command_indices)
+    ensures p.commands[next_command_indices[j]] == '-'
+    ensures new_index >= 0
+    ensures inside_the_indices(p, next_command_indices, new_index) //new_index is either greater than |p.commands| or new_index is in the indices
+    ensures new_index >= |p.commands| ==> !(new_index in next_command_indices)
+    ensures j+1 <= |next_command_indices|
+    ensures j+1 == |result|
+    ensures j+1 < |next_command_indices| ==> next_command_indices[j+1]==new_index
+    ensures matched_forall_loop(p, result, next_command_indices, j)
+    ensures in_bounds_commands(p, next_command_indices)
+    ensures loop_less_than_commands(loop_start_stack, result)
+    ensures valid_ir_commands(result)
+    ensures new_index >= 0
+    ensures |commands| >=0
+    ensures sub_changes_inclusion_1_step(p, next_command_indices)
+    ensures inside_the_indices(p, next_command_indices, new_index)
+    ensures new_index > i
+
+
+    {
+        assert matched_forall_loop(p, commands, next_command_indices, j);
+        var k:= count_consecutive_symbols(p, i);
+        var neg_k: int := k;
+        neg_k := -1*neg_k;
+        implication_with_and(p, i, k, next_command_indices); 
+        assert (i in next_command_indices && next_step(p, i, k, next_command_indices)) ==> inside_the_indices(p, next_command_indices, i+k);
+        assert i in next_command_indices ==> next_step(p, i, k, next_command_indices);
+        step_is_indices(p, i, k, next_command_indices);
+        assert (i in next_command_indices) ==> inside_the_indices(p, next_command_indices, i+k);
+        assert matched_forall_loop(p, commands, next_command_indices, j);
+
+        result := commands+ [Inc(neg_k)];
+
+        assert valid_ir_commands(result[..|result|-1]);
+        IncreasingArrayKeepsValid(result);
+        assert valid_ir_commands(result);
+
+
+        assert matched_forall_loop(p, result[..j], next_command_indices, j);
+        IncreasingArrayDoesntAffectMatching(p, result, j, next_command_indices);
+        assert matched_forall_loop(p, result, next_command_indices, j);
+
+        assert |result| >0;
+        assert (old_i in next_command_indices) ==> inside_the_indices(p, next_command_indices, i+k);
+        assert relation_between_old_new(p, old_i, i+k, next_command_indices);
+        var temp := i+k;      
+        addition_is_preserving(p, old_i, i, k, temp, next_command_indices);
+        assert relation_between_old_new(p, old_i, temp, next_command_indices);
+
+        assert temp-old_i == k;
+        assert (old_i in next_command_indices) ==> inside_the_indices(p, next_command_indices, temp);
+        assert p.commands[next_command_indices[j]] == '-';
+        assert k == count_consecutive_symbols(p, next_command_indices[j]);
+        assert neg_k <  0;
+        assert result[j] == Inc(neg_k);
+        AndIsImplicationMinus(p, result, j, next_command_indices, neg_k);
+        assert matched_command_with_ir(p, result, j, next_command_indices);
+        assert matched_forall_loop(p, result, next_command_indices, j+1);
+        assert in_bounds_commands(p, next_command_indices);
+        assert loop_less_than_commands(loop_start_stack, result);
+       new_index := temp;
+        assert just_short_length(j, next_command_indices) ==> next_command_indices[j+1] == next_command_indices[j] + count_consecutive_symbols(p, next_command_indices[j]);
+        assert j+1 < |next_command_indices| ==> next_command_indices[j+1] == i + k;
+        assert j +1 < |next_command_indices| ==> next_command_indices[j+1] == new_index;
+
+    }
+
+    method CompileRightShift(p: Program, commands: seq<Instr>, i: int, next_command_indices: seq<int>, j: int, old_i: int, loop_start_stack: seq<int>) 
+    returns (result: seq<Instr>, new_index: int)
+    requires i >= 0
+    requires valid_program(p)
+    requires next_command_indices == Changes(p)
+    requires |p.commands| > 0
+    requires |p.input| == |p.commands|
+    requires p.pointer == 0
+    requires valid_input(p.input)
+    requires |commands|>=0
+    requires changes_correct(p, next_command_indices)
+    requires sub_changes_inclusion_1_step(p, next_command_indices)
+    requires inside_the_indices(p, next_command_indices, i) //i is either greater than |p.commands| or i is in the indices
+    requires 0<=j < |next_command_indices|
+    requires j < |next_command_indices| ==> next_command_indices[j]==i
+    requires i >= |p.commands| ==> !(i in next_command_indices)
+    requires i >= |p.commands| ==> j >= |next_command_indices|
+    requires j == |commands|
+    requires old_i == i
+    requires p.commands[next_command_indices[j]] == '>'
+    requires matched_forall_loop(p, commands, next_command_indices, j)
+    requires in_bounds_commands(p, next_command_indices)
+    requires loop_less_than_commands(loop_start_stack, commands)
+    requires valid_ir_commands(commands)
+    ensures |result| == |commands|+1
+    ensures j < |result| && j < |next_command_indices|
+    ensures matched_command_with_ir(p, result, j, next_command_indices)
+    ensures matched_forall_loop(p, result, next_command_indices, j+1)
+    ensures in_bounds_commands(p, next_command_indices)
+    ensures loop_less_than_commands(loop_start_stack, result)
+    ensures valid_ir_commands(result)
+    ensures loop_less_than_commands(loop_start_stack, result)
+    ensures j== |result|-1
+    ensures matched_forall_loop(p, result, next_command_indices, j+1)
+    ensures in_bounds_commands(p, next_command_indices)
+    ensures old_i in next_command_indices ==> inside_the_indices(p, next_command_indices, new_index)
+    ensures inside_the_indices(p, next_command_indices, new_index)
+    ensures j+1 <= |next_command_indices| ==> j < |next_command_indices|
+    ensures matched_forall_loop(p, result, next_command_indices, j)
+    ensures |result| >0
+    ensures relation_between_old_new(p, old_i, new_index, next_command_indices)
+    ensures p.commands[next_command_indices[j]] == '>'
+    ensures new_index >= 0
+    ensures inside_the_indices(p, next_command_indices, new_index) //new_index is either greater than |p.commands| or new_index is in the indices
+    ensures new_index >= |p.commands| ==> !(new_index in next_command_indices)
+    ensures j+1 <= |next_command_indices|
+    ensures j+1 == |result|
+    ensures j+1 < |next_command_indices| ==> next_command_indices[j+1]==new_index
+    ensures matched_forall_loop(p, result, next_command_indices, j)
+    ensures in_bounds_commands(p, next_command_indices)
+    ensures loop_less_than_commands(loop_start_stack, result)
+    ensures valid_ir_commands(result)
+    ensures new_index >= 0
+    ensures |commands| >=0
+    ensures sub_changes_inclusion_1_step(p, next_command_indices)
+    ensures inside_the_indices(p, next_command_indices, new_index)
+    ensures new_index > i
+
+
+    {
+        assert matched_forall_loop(p, commands, next_command_indices, j);
+        var k:= count_consecutive_symbols(p, i);
+        implication_with_and(p, i, k, next_command_indices); 
+        assert (i in next_command_indices && next_step(p, i, k, next_command_indices)) ==> inside_the_indices(p, next_command_indices, i+k);
+        bigger_step_within_range(p, i, k, next_command_indices);
+        assert i in next_command_indices ==> next_step(p, i, k, next_command_indices);
+        step_is_indices(p, i, k, next_command_indices);
+        assert (i in next_command_indices) ==> inside_the_indices(p, next_command_indices, i+k);
+        assert matched_forall_loop(p, commands, next_command_indices, j);
+        assert p.commands[next_command_indices[j]] == '>';
+
+        assert valid_ir_commands(commands);
+
+        result := commands+ [Move(k)];
+
+        assert valid_ir_commands(result[..|result|-1]);
+        IncreasingArrayKeepsValidMove(result);
+        assert valid_ir_commands(result);
+
+
+        assert matched_forall_loop(p, result[..j], next_command_indices, j);
+        IncreasingArrayDoesntAffectMatching(p, result, j, next_command_indices);
+        assert matched_forall_loop(p, result, next_command_indices, j);
+
+        assert |result| >0;
+        assert (old_i in next_command_indices) ==> inside_the_indices(p, next_command_indices, i+k);
+        assert relation_between_old_new(p, old_i, i+k, next_command_indices);
+        var temp := i+k;      
+        addition_is_preserving(p, old_i, i, k, temp, next_command_indices);
+        assert relation_between_old_new(p, old_i, temp, next_command_indices);
+
+        assert temp-old_i == k;
+        assert (old_i in next_command_indices) ==> inside_the_indices(p, next_command_indices, temp);
+        assert p.commands[next_command_indices[j]] == '>';
+        assert k == count_consecutive_symbols(p, next_command_indices[j]);
+        assert k >= 0;
+        assert result[j] == Move(k);
+        AndIsImplicationMoveForwards(p, result, j, next_command_indices, k);
+
+        assert matched_command_with_ir(p, result, j, next_command_indices);
+        assert matched_forall_loop(p, result, next_command_indices, j+1);
+        assert in_bounds_commands(p, next_command_indices);
+        assert loop_less_than_commands(loop_start_stack, result);
+      new_index := temp;
+        assert just_short_length(j, next_command_indices) ==> next_command_indices[j+1] == next_command_indices[j] + count_consecutive_symbols(p, next_command_indices[j]);
+        assert j+1 < |next_command_indices| ==> next_command_indices[j+1] == i + k;
+        assert j +1 < |next_command_indices| ==> next_command_indices[j+1] == new_index;
+
+    }
+
+    method CompileLeftShift(p: Program, commands: seq<Instr>, i: int, next_command_indices: seq<int>, j: int, old_i: int, loop_start_stack: seq<int>) 
+    returns (result: seq<Instr>, new_index: int)
+    requires i >= 0
+    requires valid_program(p)
+    requires next_command_indices == Changes(p)
+    requires |p.commands| > 0
+    requires |p.input| == |p.commands|
+    requires p.pointer == 0
+    requires valid_input(p.input)
+    requires |commands|>=0
+    requires changes_correct(p, next_command_indices)
+    requires sub_changes_inclusion_1_step(p, next_command_indices)
+    requires inside_the_indices(p, next_command_indices, i) //i is either greater than |p.commands| or i is in the indices
+    requires 0<=j < |next_command_indices|
+    requires j < |next_command_indices| ==> next_command_indices[j]==i
+    requires i >= |p.commands| ==> !(i in next_command_indices)
+    requires i >= |p.commands| ==> j >= |next_command_indices|
+    requires j == |commands|
+    requires old_i == i
+    requires p.commands[next_command_indices[j]] == '<'
+    requires matched_forall_loop(p, commands, next_command_indices, j)
+    requires in_bounds_commands(p, next_command_indices)
+    requires loop_less_than_commands(loop_start_stack, commands)
+    requires valid_ir_commands(commands)
+    ensures |result| == |commands|+1
+    ensures j < |result| && j < |next_command_indices|
+    ensures matched_command_with_ir(p, result, j, next_command_indices)
+    ensures matched_forall_loop(p, result, next_command_indices, j+1)
+    ensures in_bounds_commands(p, next_command_indices)
+    ensures loop_less_than_commands(loop_start_stack, result)
+    ensures valid_ir_commands(result)
+    ensures loop_less_than_commands(loop_start_stack, result)
+    ensures j== |result|-1
+    ensures matched_forall_loop(p, result, next_command_indices, j+1)
+    ensures in_bounds_commands(p, next_command_indices)
+    ensures old_i in next_command_indices ==> inside_the_indices(p, next_command_indices, new_index)
+    ensures inside_the_indices(p, next_command_indices, new_index)
+    ensures j+1 <= |next_command_indices| ==> j < |next_command_indices|
+    ensures matched_forall_loop(p, result, next_command_indices, j)
+    ensures |result| >0
+    ensures relation_between_old_new(p, old_i, new_index, next_command_indices)
+    ensures p.commands[next_command_indices[j]] == '<'
+    ensures new_index >= 0
+    ensures inside_the_indices(p, next_command_indices, new_index) //new_index is either greater than |p.commands| or new_index is in the indices
+    ensures new_index >= |p.commands| ==> !(new_index in next_command_indices)
+    ensures j+1 <= |next_command_indices|
+    ensures j+1 == |result|
+    ensures j+1 < |next_command_indices| ==> next_command_indices[j+1]==new_index
+    ensures matched_forall_loop(p, result, next_command_indices, j)
+    ensures in_bounds_commands(p, next_command_indices)
+    ensures loop_less_than_commands(loop_start_stack, result)
+    ensures valid_ir_commands(result)
+    ensures new_index >= 0
+    ensures |commands| >=0
+    ensures sub_changes_inclusion_1_step(p, next_command_indices)
+    ensures inside_the_indices(p, next_command_indices, new_index)
+    ensures new_index > i
+
+
+    {
+        assert matched_forall_loop(p, commands, next_command_indices, j);
+        var k:= count_consecutive_symbols(p, i);
+        var neg_k: int := k;
+        neg_k := -1*neg_k;
+        implication_with_and(p, i, k, next_command_indices); 
+        assert (i in next_command_indices && next_step(p, i, k, next_command_indices)) ==> inside_the_indices(p, next_command_indices, i+k);
+        bigger_step_within_range(p, i, k, next_command_indices);
+        step_is_indices(p, i, k, next_command_indices);
+        assert (i in next_command_indices) ==> inside_the_indices(p, next_command_indices, i+k);
+        assert matched_forall_loop(p, commands, next_command_indices, j);
+
+        assert valid_ir_commands(commands);
+        
+        result := commands+ [Move(neg_k)];
+
+        assert valid_ir_commands(result[..|result|-1]);
+        IncreasingArrayKeepsValidMove(result);
+        assert valid_ir_commands(result);
+
+        assert matched_forall_loop(p, result[..j], next_command_indices, j);
+        IncreasingArrayDoesntAffectMatching(p, result, j, next_command_indices);
+        assert matched_forall_loop(p, result, next_command_indices, j);
+
+        assert |result| >0;
+        assert (old_i in next_command_indices) ==> inside_the_indices(p, next_command_indices, i+k);
+        assert relation_between_old_new(p, old_i, i+k, next_command_indices);
+        var temp := i+k;      
+        addition_is_preserving(p, old_i, i, k, temp, next_command_indices);
+        assert relation_between_old_new(p, old_i, temp, next_command_indices);
+
+        assert temp-old_i == k;
+        assert (old_i in next_command_indices) ==> inside_the_indices(p, next_command_indices, temp);
+        assert p.commands[next_command_indices[j]] == '<';
+        assert k == count_consecutive_symbols(p, next_command_indices[j]);
+        assert neg_k <  0;
+        assert result[j] == Move(neg_k);
+        AndIsImplicationMoveBackwards(p, result, j, next_command_indices, neg_k);
+        assert matched_command_with_ir(p, result, j, next_command_indices);
+        assert matched_forall_loop(p, result, next_command_indices, j+1);
+        assert in_bounds_commands(p, next_command_indices);
+        assert loop_less_than_commands(loop_start_stack, result);
+        new_index := temp;
+        assert just_short_length(j, next_command_indices) ==> next_command_indices[j+1] == next_command_indices[j] + count_consecutive_symbols(p, next_command_indices[j]);
+        assert j+1 < |next_command_indices| ==> next_command_indices[j+1] == i + k;
+        assert j +1 < |next_command_indices| ==> next_command_indices[j+1] == new_index;
+
+    }
+    method CompileTrueJump(p: Program, commands: seq<Instr>, i: int, next_command_indices: seq<int>, j: int, old_i: int, loop_start_stack: seq<int>) 
+    returns (result: seq<Instr>, new_index: int)
+    requires i >= 0
+    requires valid_program(p)
+    requires next_command_indices == Changes(p)
+    requires |p.commands| > 0
+    requires |p.input| == |p.commands|
+    requires p.pointer == 0
+    requires valid_input(p.input)
+    requires |commands|>=0
+    requires changes_correct(p, next_command_indices)
+    requires sub_changes_inclusion_1_step(p, next_command_indices)
+    requires inside_the_indices(p, next_command_indices, i) //i is either greater than |p.commands| or i is in the indices
+    requires 0<=j < |next_command_indices|
+    requires j < |next_command_indices| ==> next_command_indices[j]==i
+    requires i >= |p.commands| ==> !(i in next_command_indices)
+    requires i >= |p.commands| ==> j >= |next_command_indices|
+    requires j == |commands|
+    requires old_i == i
+    requires p.commands[next_command_indices[j]] == '['
+    requires matched_forall_loop(p, commands, next_command_indices, j)
+    requires in_bounds_commands(p, next_command_indices)
+    requires loop_less_than_commands(loop_start_stack, commands)
+    requires valid_ir_commands(commands)
+    ensures |result| == |commands|+1
+    ensures j < |result| && j < |next_command_indices|
+    ensures matched_command_with_ir(p, result, j, next_command_indices)
+    ensures matched_forall_loop(p, result, next_command_indices, j+1)
+    ensures in_bounds_commands(p, next_command_indices)
+    ensures loop_less_than_commands(loop_start_stack, result)
+    ensures valid_ir_commands(result)
+    ensures loop_less_than_commands(loop_start_stack, result)
+    ensures j== |result|-1
+    ensures matched_forall_loop(p, result, next_command_indices, j+1)
+    ensures in_bounds_commands(p, next_command_indices)
+    ensures old_i in next_command_indices ==> inside_the_indices(p, next_command_indices, new_index)
+    ensures inside_the_indices(p, next_command_indices, new_index)
+    ensures j+1 <= |next_command_indices| ==> j < |next_command_indices|
+    ensures matched_forall_loop(p, result, next_command_indices, j)
+    ensures |result| >0
+    ensures relation_between_old_new(p, old_i, new_index, next_command_indices)
+    ensures p.commands[next_command_indices[j]] == '['
+    ensures new_index >= 0
+    ensures inside_the_indices(p, next_command_indices, new_index) //new_index is either greater than |p.commands| or new_index is in the indices
+    ensures new_index >= |p.commands| ==> !(new_index in next_command_indices)
+    ensures j+1 <= |next_command_indices|
+    ensures j+1 == |result|
+    ensures j+1 < |next_command_indices| ==> next_command_indices[j+1]==new_index
+    ensures matched_forall_loop(p, result, next_command_indices, j)
+    ensures in_bounds_commands(p, next_command_indices)
+    ensures loop_less_than_commands(loop_start_stack, result)
+    ensures valid_ir_commands(result)
+    ensures new_index >= 0
+    ensures |commands| >=0
+    ensures sub_changes_inclusion_1_step(p, next_command_indices)
+    ensures inside_the_indices(p, next_command_indices, new_index)
+    ensures new_index > i
+    ensures result[|result|-1] == Jump(0, true)
+
+
+    {
+        var k := 1;
+        assert p.commands[next_command_indices[j]] == '[';
+        assert j == |commands|;
+        assert valid_ir_commands(commands);
+        result := commands+ [Jump(0, true)];
+
+
+        assert result[|result|-1] == Jump(0, true);
+        assert valid_ir_commands(result[..|result|-1]);
+        IncreasingArrayKeepsValidJumpOne(result);
+        assert valid_ir_commands(result);
+        assert j == |result|-1;
+        assert result[j] == Jump(0, true);
+        assert |result| >0;
+        assert matched_forall_loop(p, result[..j], next_command_indices, j);
+        IncreasingArrayDoesntAffectMatching(p, result, j, next_command_indices);
+        assert matched_forall_loop(p, result, next_command_indices, j);
+        assert (old_i in next_command_indices) ==> inside_the_indices(p, next_command_indices, i+k);
+        assert relation_between_old_new(p, old_i, i+k, next_command_indices);
+
+        var temp := i+k;      
+        addition_is_preserving(p, old_i, i, k, temp, next_command_indices);
+        assert relation_between_old_new(p, old_i, temp, next_command_indices);
+        assert temp-old_i == k;
+        single_step_within_range(p, old_i, k, next_command_indices);
+
+        assert (old_i in next_command_indices) ==> inside_the_indices(p, next_command_indices, temp);
+
+        assert p.commands[next_command_indices[j]] == '[';
+        simple_exclusion_2(p.commands[next_command_indices[j]]);
+        assert !(p.commands[next_command_indices[j]] in ['+', '-', '<', '>']);
+        assert result[j] == Jump(0, true);
+        assert result[|result|-1] == Jump(0, true);
+        assert 0<= j < |result|;
+        assert 0<= j < |next_command_indices|;
+        assert 0<= next_command_indices[j] < |p.commands|;
+        // assume matched_forall_loop(p, result, next_command_indices, j);
+        AndIsImplicationJumpFor(p, result, j, next_command_indices, 0);
+        assert matched_forall_loop(p, result, next_command_indices, j+1);
+        new_index := temp;
+        assert just_short_length(j, next_command_indices) ==> next_command_indices[j+1] == next_command_indices[j] + 1;
+        assert j+1 < |next_command_indices| ==> next_command_indices[j+1] == i + k;
+        assert j +1 < |next_command_indices| ==> next_command_indices[j+1] == new_index;
+
+    }
+
+
+    method CompileFalseJump(p: Program, commands: seq<Instr>, i: int, next_command_indices: seq<int>, j: int, old_i: int, loop_start_stack: seq<int>) 
+    returns (result: seq<Instr>, new_index: int)
+    requires i >= 0
+    requires valid_program(p)
+    requires next_command_indices == Changes(p)
+    requires |p.commands| > 0
+    requires |p.input| == |p.commands|
+    requires p.pointer == 0
+    requires valid_input(p.input)
+    requires |commands|>=0
+    requires changes_correct(p, next_command_indices)
+    requires sub_changes_inclusion_1_step(p, next_command_indices)
+    requires inside_the_indices(p, next_command_indices, i) //i is either greater than |p.commands| or i is in the indices
+    requires 0<=j < |next_command_indices|
+    requires j < |next_command_indices| ==> next_command_indices[j]==i
+    requires i >= |p.commands| ==> !(i in next_command_indices)
+    requires i >= |p.commands| ==> j >= |next_command_indices|
+    requires j == |commands|
+    requires old_i == i
+    requires p.commands[next_command_indices[j]] == ']'
+    requires matched_forall_loop(p, commands, next_command_indices, j)
+    requires in_bounds_commands(p, next_command_indices)
+    requires loop_less_than_commands(loop_start_stack, commands)
+    requires valid_ir_commands(commands)
+    ensures |result| == |commands|+1
+    ensures j < |result| && j < |next_command_indices|
+    ensures matched_command_with_ir(p, result, j, next_command_indices)
+    ensures matched_forall_loop(p, result, next_command_indices, j+1)
+    ensures in_bounds_commands(p, next_command_indices)
+    ensures loop_less_than_commands(loop_start_stack, result)
+    ensures valid_ir_commands(result)
+    ensures loop_less_than_commands(loop_start_stack, result)
+    ensures j== |result|-1
+    ensures matched_forall_loop(p, result, next_command_indices, j+1)
+    ensures in_bounds_commands(p, next_command_indices)
+    ensures old_i in next_command_indices ==> inside_the_indices(p, next_command_indices, new_index)
+    ensures inside_the_indices(p, next_command_indices, new_index)
+    ensures j+1 <= |next_command_indices| ==> j < |next_command_indices|
+    ensures matched_forall_loop(p, result, next_command_indices, j)
+    ensures |result| >0
+    ensures relation_between_old_new(p, old_i, new_index, next_command_indices)
+    ensures p.commands[next_command_indices[j]] == ']'
+    ensures new_index >= 0
+    ensures inside_the_indices(p, next_command_indices, new_index) //new_index is either greater than |p.commands| or new_index is in the indices
+    ensures new_index >= |p.commands| ==> !(new_index in next_command_indices)
+    ensures j+1 <= |next_command_indices|
+    ensures j+1 == |result|
+    ensures j+1 < |next_command_indices| ==> next_command_indices[j+1]==new_index
+    ensures matched_forall_loop(p, result, next_command_indices, j)
+    ensures in_bounds_commands(p, next_command_indices)
+    ensures loop_less_than_commands(loop_start_stack, result)
+    ensures valid_ir_commands(result)
+    ensures new_index >= 0
+    ensures |commands| >=0
+    ensures sub_changes_inclusion_1_step(p, next_command_indices)
+    ensures inside_the_indices(p, next_command_indices, new_index)
+    ensures new_index > i
+    ensures result[|result|-1] == Jump(0, false)
+
+
+    {
+        var k := 1;
+        assert p.commands[next_command_indices[j]] == ']';
+        assert j == |commands|;
+        assert valid_ir_commands(commands);
+        result := commands+ [Jump(0, false)];
+
+
+        assert result[|result|-1] == Jump(0, false);
+        assert valid_ir_commands(result[..|result|-1]);
+        IncreasingArrayKeepsValidJumpTwo(result);
+        assert valid_ir_commands(result);
+        assert j == |result|-1;
+        assert result[j] == Jump(0, false);
+        assert |result| >0;
+        assert matched_forall_loop(p, result[..j], next_command_indices, j);
+        IncreasingArrayDoesntAffectMatching(p, result, j, next_command_indices);
+        assert matched_forall_loop(p, result, next_command_indices, j);
+        assert (old_i in next_command_indices) ==> inside_the_indices(p, next_command_indices, i+k);
+        assert relation_between_old_new(p, old_i, i+k, next_command_indices);
+        var temp := i+k;      
+        addition_is_preserving(p, old_i, i, k, temp, next_command_indices);
+        assert relation_between_old_new(p, old_i, temp, next_command_indices);
+        assert temp-old_i == k;
+        single_step_within_range_close_loop(p, old_i, k, next_command_indices);
+
+        assert (old_i in next_command_indices) ==> inside_the_indices(p, next_command_indices, temp);
+
+        assert p.commands[next_command_indices[j]] == ']';
+        simple_exclusion(p.commands[next_command_indices[j]]);
+        assert !(p.commands[next_command_indices[j]] in ['+', '-', '<', '>']);
+        assert result[j] == Jump(0, false);
+        assert result[|result|-1] == Jump(0, false);
+        assert 0<= j < |result|;
+        assert 0<= j < |next_command_indices|;
+        assert 0<= next_command_indices[j] < |p.commands|;
+        AndIsImplicationJumpBack(p, result, j, next_command_indices, 0);
+        assert matched_forall_loop(p, result, next_command_indices, j+1);
+        assert loop_less_than_commands(loop_start_stack, result);
+        new_index := temp;
+        assert just_short_length(j, next_command_indices) ==> next_command_indices[j+1] == next_command_indices[j] + 1;
+        assert j+1 < |next_command_indices| ==> next_command_indices[j+1] == i + k;
+        assert j +1 < |next_command_indices| ==> next_command_indices[j+1] == new_index;
+
+    }
+
+    method CompileIO(p: Program, commands: seq<Instr>, i: int, next_command_indices: seq<int>, j: int, old_i: int, loop_start_stack: seq<int>) 
+    returns (result: seq<Instr>, new_index: int)
+    requires i >= 0
+    requires valid_program(p)
+    requires next_command_indices == Changes(p)
+    requires |p.commands| > 0
+    requires |p.input| == |p.commands|
+    requires p.pointer == 0
+    requires valid_input(p.input)
+    requires |commands|>=0
+    requires changes_correct(p, next_command_indices)
+    requires sub_changes_inclusion_1_step(p, next_command_indices)
+    requires inside_the_indices(p, next_command_indices, i) //i is either greater than |p.commands| or i is in the indices
+    requires 0<=j < |next_command_indices|
+    requires j < |next_command_indices| ==> next_command_indices[j]==i
+    requires i >= |p.commands| ==> !(i in next_command_indices)
+    requires i >= |p.commands| ==> j >= |next_command_indices|
+    requires j == |commands|
+    requires old_i == i
+    requires p.commands[next_command_indices[j]] == ',' || p.commands[next_command_indices[j]] == '.'
+    requires matched_forall_loop(p, commands, next_command_indices, j)
+    requires in_bounds_commands(p, next_command_indices)
+    requires loop_less_than_commands(loop_start_stack, commands)
+    requires valid_ir_commands(commands)
+    ensures |result| == |commands|+1
+    ensures j < |result| && j < |next_command_indices|
+    ensures matched_command_with_ir(p, result, j, next_command_indices)
+    ensures matched_forall_loop(p, result, next_command_indices, j+1)
+    ensures in_bounds_commands(p, next_command_indices)
+    ensures loop_less_than_commands(loop_start_stack, result)
+    ensures valid_ir_commands(result)
+    ensures loop_less_than_commands(loop_start_stack, result)
+    ensures j== |result|-1
+    ensures matched_forall_loop(p, result, next_command_indices, j+1)
+    ensures in_bounds_commands(p, next_command_indices)
+    ensures old_i in next_command_indices ==> inside_the_indices(p, next_command_indices, new_index)
+    ensures inside_the_indices(p, next_command_indices, new_index)
+    ensures j+1 <= |next_command_indices| ==> j < |next_command_indices|
+    ensures matched_forall_loop(p, result, next_command_indices, j)
+    ensures |result| >0
+    ensures relation_between_old_new(p, old_i, new_index, next_command_indices)
+    ensures p.commands[next_command_indices[j]] == ',' || p.commands[next_command_indices[j]] == '.'
+    ensures new_index >= 0
+    ensures inside_the_indices(p, next_command_indices, new_index) //new_index is either greater than |p.commands| or new_index is in the indices
+    ensures new_index >= |p.commands| ==> !(new_index in next_command_indices)
+    ensures j+1 <= |next_command_indices|
+    ensures j+1 == |result|
+    ensures j+1 < |next_command_indices| ==> next_command_indices[j+1]==new_index
+    ensures matched_forall_loop(p, result, next_command_indices, j)
+    ensures in_bounds_commands(p, next_command_indices)
+    ensures loop_less_than_commands(loop_start_stack, result)
+    ensures valid_ir_commands(result)
+    ensures new_index >= 0
+    ensures |commands| >=0
+    ensures sub_changes_inclusion_1_step(p, next_command_indices)
+    ensures inside_the_indices(p, next_command_indices, new_index)
+    ensures new_index > i
+
+
+    {
+        assert matched_forall_loop(p, commands, next_command_indices, j);
+        var k:= 1;
+        implication_with_and(p, i, k, next_command_indices); 
+        assert (i in next_command_indices && next_step(p, i, k, next_command_indices)) ==> inside_the_indices(p, next_command_indices, i+k);
+        single_step_within_range(p, i, k, next_command_indices);
+        step_is_indices(p, i, k, next_command_indices);
+        assert (i in next_command_indices) ==> inside_the_indices(p, next_command_indices, i+k);
+        assert matched_forall_loop(p, commands, next_command_indices, j);
+
+        if p.commands[next_command_indices[j]]== '.'{
+          result := commands+ [Print];
+          assert valid_ir_commands(result[..|result|-1]);
+          IncreasingArrayKeepsValidIO(result);
+          assert valid_ir_commands(result);
+
+          assert |result| >0;
+          assert matched_forall_loop(p, result[..j], next_command_indices, j);
+          IncreasingArrayDoesntAffectMatching(p, result, j, next_command_indices);
+          assert matched_forall_loop(p, result, next_command_indices, j);
+          assert (old_i in next_command_indices) ==> inside_the_indices(p, next_command_indices, i+k);
+          assert relation_between_old_new(p, old_i, i+k, next_command_indices);
+
+          var temp := i+k;      
+          addition_is_preserving(p, old_i, i, k, temp, next_command_indices);
+          assert relation_between_old_new(p, old_i, temp, next_command_indices);
+          assert temp-old_i == k;
+          single_step_within_range(p, old_i, k, next_command_indices);
+
+          assert (old_i in next_command_indices) ==> inside_the_indices(p, next_command_indices, temp);
+          simple_exclusion(p.commands[next_command_indices[j]]);
+          assert !(p.commands[next_command_indices[j]] in ['+', '-', '<', '>']);
+          assert result[j] == Print;
+          AndIsImplicationPrint(p, result, j, next_command_indices);
+          new_index := temp;
+          assert just_short_length(j, next_command_indices) ==> next_command_indices[j+1] == next_command_indices[j] + 1;
+          assert j+1 < |next_command_indices| ==> next_command_indices[j+1] == i + k;
+          assert j +1 < |next_command_indices| ==> next_command_indices[j+1] == new_index;
+
+          
+        } else{
+          assert p.commands[next_command_indices[j]] == ',';
+          result := commands+ [UserInput];
+          assert valid_ir_commands(result[..|result|-1]);
+          IncreasingArrayKeepsValidIO(result);
+          assert valid_ir_commands(result);
+
+          assert |result| >0;
+
+          assert matched_forall_loop(p, result[..j], next_command_indices, j);
+          IncreasingArrayDoesntAffectMatching(p, result, j, next_command_indices);
+          assert matched_forall_loop(p, result, next_command_indices, j);
+          assert (old_i in next_command_indices) ==> inside_the_indices(p, next_command_indices, i+k);
+          assert relation_between_old_new(p, old_i, i+k, next_command_indices);
+
+          var temp := i+k;      
+          addition_is_preserving(p, old_i, i, k, temp, next_command_indices);
+          assert relation_between_old_new(p, old_i, temp, next_command_indices);
+          assert temp-old_i == k;
+          single_step_within_range(p, old_i, k, next_command_indices);
+
+          assert (old_i in next_command_indices) ==> inside_the_indices(p, next_command_indices, temp);
+          assert p.commands[next_command_indices[j]] == ',';
+          simple_exclusion_2(p.commands[next_command_indices[j]]);
+          assert !(p.commands[next_command_indices[j]] in ['+', '-', '<', '>']);
+          assert result[j] == UserInput;
+          AndIsImplicationInput(p, result, j, next_command_indices);
+        new_index := temp;
+        assert just_short_length(j, next_command_indices) ==> next_command_indices[j+1] == next_command_indices[j] + 1;
+        assert j+1 < |next_command_indices| ==> next_command_indices[j+1] == i + k;
+        assert j +1 < |next_command_indices| ==> next_command_indices[j+1] == new_index;
+
+
+          
+        }
+  
+        assert matched_command_with_ir(p, result, j, next_command_indices);
+        assert matched_forall_loop(p, result, next_command_indices, j+1);
+        assert in_bounds_commands(p, next_command_indices);
+        assert loop_less_than_commands(loop_start_stack, result);
+        
+
+
+    }
+
+
+}
