equivalence.dfy
@@ -7,39 +7,6 @@ module Equivalence{
     // import opened Lemmas
     import opened Common
     import opened Steps
-    // ghost predicate AreEquivalent(bf_program: Program, bf_state: State, ir_program: IntermediateRep, input: seq<char>, inputPtr: int)
-    // requires 0 <= bf_program.pointer <= |bf_program.commands|
-    // requires 0 <= bf_state.pointer < |bf_state.memory| 
-    // decreases |bf_program.commands|- bf_program.pointer
-    // requires 0 <= inputPtr <= |input|
-    // requires valid_program(bf_program) 
-    // requires state_reqs(bf_state)
-    // ensures !(bf_program.pointer >= |bf_program.commands| && !(ir_program.pointer >= |ir_program.commands|)) || !(!(bf_program.pointer >= |bf_program.commands|) && (ir_program.pointer >= |ir_program.commands|))
-    //     {
-    //         if bf_program.pointer >= |bf_program.commands| && ir_program.pointer >= |ir_program.commands| then
-    //             true
-    //         else if !(bf_program.pointer >= |bf_program.commands| && !(ir_program.pointer >= |ir_program.commands|)) || !(!(bf_program.pointer >= |bf_program.commands|) && (ir_program.pointer >= |ir_program.commands|)) then
-    //         // else 
-    //             // exists i: int :: true
-    //             // true
-    //             exists next_bf_state: State, next_bf_program: Program, next_ir: IntermediateRep, postPtr: int:: 
-    //             0<=bf_program.pointer < next_bf_program.pointer <= |next_bf_program.commands| &&
-    //             0 <= ir_program.pointer < next_ir.pointer <= |ir_program.commands| &&
-    //             inputPtr <= postPtr <= |input| &&
-
-    //             next_ir.commands == ir_program.commands && bf_program.commands == next_bf_program.commands
-    //             &&
-    //             state_reqs(next_bf_state)
-    //             &&
-    //             |next_bf_state.memory| == |bf_state.memory|
-    //             // &&
-    //             && 0<=next_bf_state.pointer < |next_bf_state.memory| 
-    //             && max_steps(bf_program, bf_state, next_bf_program, next_bf_state)
-    //             && ir_step(ir_program, bf_state, next_ir, next_bf_state) && AreEquivalent(next_bf_program, next_bf_state, next_ir, input, postPtr)
-            
-    //         else
-    //             false 
-    //     }
 
     ghost predicate equiv_locations(p: Program, ir: IntermediateRep)
     {
@@ -121,10 +88,6 @@ ghost predicate aligned_instructions_subseq(p: Program, ir: seq<Instr>)
             0<=Changes(p)[i] < |p.commands| &&
             matched_command_with_ir(p, ir, i, Changes(p))
         )
-        // (p.pointer == |p.commands| && ir.pointer == |ir.commands|) ||
-        // (p.pointer < |p.commands| && ir.pointer < |ir.commands| &&
-        
-        //  )
     } 
 
 
@@ -138,10 +101,7 @@ ghost predicate aligned_instructions(p: Program, ir: IntermediateRep)
             0<=Changes(p)[i] < |p.commands| &&
             matched_command_with_ir(p, ir.commands, i, Changes(p))
         )
-        // (p.pointer == |p.commands| && ir.pointer == |ir.commands|) ||
-        // (p.pointer < |p.commands| && ir.pointer < |ir.commands| &&
-        
-        //  )
+
     } 
 
 }
